Some work on shard clerk proof

src/program_proof/memkv/memkv_shard_clerk_proof.v
@@ -19,13 +19,53 @@ Record GetReplyC := {
 Axiom has_encoding_GetRequest : (list u8) → GetRequestC → Prop.
 Axiom has_encoding_GetReply : (list u8) → GetReplyC → Prop.
 
-Context `{!heapG Σ, rpcG Σ GetReply}.
+Context `{!heapG Σ, rpcG Σ GetReplyC}.
 
+Lemma wp_encodeGetRequest (cid seq key:u64) :
+  {{{
+       True
+  }}}
+    encodeGetRequest (#cid, (#seq, (#key, #())))%V
+  {{{
+       (reqData:list u8) req_sl, RET (slice_val req_sl); ⌜has_encoding_GetRequest reqData {| GR_CID:=cid; GR_Seq:=seq; GR_Key:=key |}⌝ ∗
+                                               typed_slice.is_slice req_sl byteT 1%Qp reqData
+  }}}.
+Proof.
+Admitted.
 
-Definition uKV_GET := 3.
-Definition is_shard_server host : iProp Σ :=
-  "HgetSpec" ∷ handler_is (list u8) host uKV_GET
-             (λ x reqData, True ) (* pre *)
+Lemma wp_decodeGetReply rep rep_sl repData :
+  {{{
+       typed_slice.is_slice rep_sl byteT 1%Qp repData ∗
+       ⌜has_encoding_GetReply repData rep ⌝
+  }}}
+    decodeGetReply (slice_val rep_sl)
+  {{{
+       (rep_ptr:loc) val_sl, RET #rep_ptr;
+       rep_ptr ↦[GetReply.S :: "Err"] #rep.(GR_Err) ∗
+       rep_ptr ↦[GetReply.S :: "Value"] (slice_val val_sl) ∗
+       typed_slice.is_slice val_sl byteT 1%Qp rep.(GR_Value)
+  }}}.
+Proof.
+Admitted.
+
+Record memkv_shard_names := {
+ rpc_gn : rpc_names ;
+ kv_gn : gname
+}
+.
+
+Implicit Type γ : memkv_shard_names.
+
+Axiom kvptsto : gname → u64 → list u8 → iProp Σ.
+
+Definition uKV_GET := 2.
+Definition is_shard_server host γ : iProp Σ :=
+  "HgetSpec" ∷ handler_is (list u8 * rpc_request_names) host uKV_GET
+             (λ x reqData, ∃ req, ⌜has_encoding_GetRequest reqData req⌝ ∗
+                                   is_RPCRequest γ.(rpc_gn) x.2 (kvptsto γ.(kv_gn) req.(GR_Key) x.1) (λ rep,
+                                                                                           ⌜rep.(GR_Value) = x.1⌝ ∗
+                                                                                           kvptsto γ.(kv_gn) req.(GR_Key) x.1) {| Req_CID:=req.(GR_CID); Req_Seq:=req.(GR_Seq) |}
+             ) (* pre *)
              (λ x reqData repData, ∃ req rep, ⌜has_encoding_GetReply repData rep⌝ ∗
                                               ⌜has_encoding_GetRequest reqData req⌝
                                               (* RPCReplyReceipt γ.(rpc_gn) req.CID req.Seq *)
@@ -50,25 +90,21 @@ Meanwhile, client keeps a fupd
 
 *)
 
-Record memkv_shard_names := {
- rpc_gn : rpc_names ;
- kv_gn : gname
-}
-.
-
-Implicit Type γ : memkv_shard_names.
-
 Definition own_MemKVShardClerk (ck:loc) γ : iProp Σ :=
-  ∃ cid seq,
-    RPCClient_own_ghost γ.(rpc_gn) cid seq
+  ∃ (cid seq:u64) (cl:loc) (host:string),
+    "Hcid" ∷ ck ↦[MemKVShardClerk.S :: "cid"] #cid ∗
+    "Hseq" ∷ ck ↦[MemKVShardClerk.S :: "seq"] #seq ∗
+    "Hcl" ∷ ck ↦[MemKVShardClerk.S :: "cl"] #cl ∗
+    "Hcrpc" ∷ RPCClient_own_ghost γ.(rpc_gn) cid seq ∗
+    "Hcl_own" ∷ grove_ffi.RPCClient_own cl host ∗
+    "#His_shard" ∷ is_shard_server host γ
 .
-
-Axiom kvptsto : gname → u64 → list u8 → iProp Σ.
 
 Lemma wp_MemKVShardClerk__Get γ (ck:loc) (key:u64) (v:list u8) (value_ptr:loc) :
   {{{
        kvptsto γ.(kv_gn) key v ∗
-       own_MemKVShardClerk ck γ
+       own_MemKVShardClerk ck γ ∗
+       (∃ dummy_sl, value_ptr ↦[slice.T byteT] (slice_val dummy_sl))
   }}}
     MemKVShardClerk__Get #ck #key #value_ptr
   {{{
@@ -77,8 +113,74 @@ Lemma wp_MemKVShardClerk__Get γ (ck:loc) (key:u64) (v:list u8) (value_ptr:loc) 
 .
 Proof.
   iIntros (Φ) "Hpre HΦ".
+  iDestruct "Hpre" as "(Hkvptsto & Hck & Hval)".
+  iNamed "Hck".
   wp_lam.
   wp_pures.
+  wp_loadField.
+  wp_loadField.
+
+  wp_pures.
+  wp_loadField.
+  wp_storeField.
+
+  wp_apply (wp_ref_of_zero).
+  { done. }
+  iIntros (rawRep) "HrawRep".
+  wp_pures.
+
+  iAssert (∃ rep_sl, rawRep ↦[slice.T byteT] (slice_val rep_sl) )%I with "[HrawRep]" as "HrawRep".
+  {
+    iExists _; iFrame.
+    admit.
+  }
+  iAssert (True)%I with "[Hkvptsto]" as "_".
+  { done. }
+  wp_forBreak_cond.
+  iNamed "HrawRep".
+  wp_pures.
+
+  wp_apply (wp_encodeGetRequest).
+  iIntros (reqData req_sl) "[%HencReq Hreq_sl]".
+  wp_loadField.
+
+  unfold is_shard_server.
+  wp_apply (wp_RPCClient__Call with "[$His_shard $Hreq_sl $HrawRep $Hcl_own]").
+  {
+    admit.
+  }
+  iIntros (b rep_sl' repData) "HcallPost".
+  wp_if_destruct.
+  {
+    wp_pures.
+    iModIntro.
+    iLeft.
+    iFrame.
+    iDestruct "HcallPost" as "(HrawRep & $ & HcallPost)".
+    iSplitL ""; first done.
+    iExists _; iFrame "HrawRep".
+  }
+  {
+    iModIntro.
+    iRight.
+    iSplitL ""; first done.
+    wp_pures.
+    iDestruct "HcallPost" as "(HrawRep & Hcl_own & Hreq_sl & Hrep_sl & [%Hbad | HcallPost ])".
+    { exfalso. naive_solver. }
+    iDestruct "HcallPost" as "(_ & >Hpost)".
+    wp_load.
+    iDestruct "Hpost" as (??) "[% %]".
+    wp_apply (wp_decodeGetReply with "[$Hrep_sl]").
+    { done. }
+    iIntros (??) "(HrepErr & HrepValue & HrepValue_sl)".
+    wp_pures.
+    wp_loadField.
+    iNamed "Hval".
+    wp_store.
+    wp_loadField.
+    iApply "HΦ".
+    done.
+  }
 Admitted.
 
 End memkv_shard_clerk_proof.
